cleanedup version

examples/Online_with_authn/DY.OnlineA.Authn.fst
@@ -9,6 +9,12 @@ open DY.Extend
 open DY.OnlineA.Data
 open DY.OnlineA.Invariants
 
+/// This is the new property, we want to show:
+/// if Alice finishes a run identified by Bob and a nonce n_a,
+/// then this Bob was involved in the run,
+/// i.e., Bob sent n_a in an acknowledgement to Alice.
+/// Unless one of Alice or Bob are corrupt.
+
 val authn:
   tr:trace -> 
   alice:principal -> bob:principal ->
@@ -23,3 +29,20 @@ val authn:
      state_was_set_some_id tr bob (SendingAck {alice; n_a})
   )
 let authn tr alice bob n_a = ()
+
+
+/// We still have nonce secrecy:
+
+val n_a_secrecy:
+  tr:trace -> alice:principal -> bob:principal -> n_a:bytes ->
+  Lemma
+  (requires
+    attacker_knows tr n_a /\
+    trace_invariant tr /\ (
+      (exists sess_id. state_was_set tr alice sess_id (SendingPing {bob; n_a})) \/
+      (exists sess_id. state_was_set tr alice sess_id (ReceivedAck {bob; n_a} ))
+    )
+  )
+  (ensures is_corrupt tr (principal_label alice) \/ is_corrupt tr (principal_label bob))
+let n_a_secrecy tr alice bob n_a =
+  attacker_only_knows_publishable_values tr n_a
