examples/Online_with_authn/DY.OnlineA.Invariants.Proofs.fst
@@ -20,196 +20,10 @@ open DY.OnlineA.Invariants
 /// For every step s we show a lemma of the form:
 /// trace_invariant tr ==> trace_invariant ( trace after step s )
 
+/// Again, we will only highlight the differences to the proofs for the secrecy model.
 
 (*** Sending a Ping maintains the invariants ***)
 
-
-/// The invariant lemma for the first step `send_ping`
-
-val send_ping_invariant:
-  alice:principal -> bob:principal -> keys_sid:state_id ->
-  tr:trace ->
-  Lemma
-  ( requires trace_invariant tr
-  )
-  (ensures (
-    let (_ , tr_out) = send_ping alice bob keys_sid tr in
-    trace_invariant tr_out
-  ))
-(* The proof works by showing that the trace invariant is maintained
-   by every traceful action in the step.
-   So we replicate the actions of the step and show trace_invariant after each.
-   
-   (Note that we are now in the "Lemma context",
-   so we have to unfold the monadic lets and sequences.)
-*)
-let send_ping_invariant alice bob keys_sid  tr =
-  (* The first action is generating the nonce n_a.
-  
-     Note that we can't use let* here since we are not in the traceful monad.
-     Thus, we have to pass the trace `tr` explicitly as last argument.
-     And we get back the new trace `tr_rand`.
-  *)
-  let (n_a, tr_rand) = gen_rand_labeled (nonce_label alice bob) tr in
-  (* That the trace invariant holds after this action,
-     can be shown automatically.
-
-     There is a corresponding lemma in `DY.Core.Trace.Manipulation`:
-     `mk_rand_trace_invariant`.
-     It comes with an SMT Pattern an hence is applied automatically.
-  *)
-  assert(trace_invariant tr_rand);
-
-  let (_, tr_ev) = trigger_event alice (Initiating {alice; bob; n_a}) tr_rand in
-
-  // Defining the abstract message does not change the trace,
-  // so we don't have to show anything.
-  let ping = Ping {alice; n_a} in 
-
- (* The last traceful action in this step is starting a new session *)
-      let st = SendingPing {bob; n_a} in
-      let (sid, tr_sess) = start_new_session alice st tr_ev in
-      (* `start_new_session` is just calling `new_session_id` and then `set_state`.
-         So we have to check that both of those maintain the trace invariant.
-
-         For `new_session_id` we find the lemma 
-         `new_session_id_same_trace` in `DY.Core.Trace.Manipulation`
-         which says that the trace is not changed.
-         Hence it trivially maintains the trace invariant.
-         It comes with an SMT pattern, so it is applied automatically.
-
-         In the same file, we have the lemma `set_state_invariant`,
-         which gives an additional pre-condition 
-         for when the trace after the state was set satisfies the trace invariant.
-         This pre-condition is that the new state must satisfy the state predicate.
-
-         The state predicate for the SendingPing state requires that
-         the nonce stored in the state has the label `nonce_label alice' bob'`, where
-         * alice' is the storing principal
-         * bob' is the name stored in the first component of the state
-
-         Similarly to above,
-         we generated the nonce wit the label `nonce_label alice bob` and
-         alice is storing the new state, and
-         bob is stored in the first component of the state.
-         So the state prediate is satisfied:
-      *)
-      assert(state_predicate_p.pred tr_ev alice sid st);
-      (* With this, we have all pre-conditions of `set_state_invariant`.
-         Since that lemma comes with an SMT pattern,
-         it is applied automatically.
-      *)
-      assert(trace_invariant tr_sess);
-
-  (* The call of `pke_enc_for` in the traceful + option monad 
-     has to be unfolded:
-     * We pass the current trace `tr_rand` as las argument
-     * We need to make a case distinction on the resulting option
-       and show trace_invariant in each case separately
-  *)
-  match pke_enc_for alice bob keys_sid key_tag ping tr_sess with
-  | (None, _) -> ( 
-      (* If encryption fails, the trace is not changed,
-         and hence the resulting trace after send_ping is tr_rand.
-         Since we already showed trace_invariant for tr_rand,
-         we don't have to show anything else in this case.
-
-        If you want to check this,
-        you can uncomment the next lines
-      *)
-      // let (_ , tr_out) = send_ping alice bob keys_sid tr in 
-      // assert(tr_out == tr_rand);
-      // assert(trace_invariant tr_out);
-      ()
-    )
-  | (Some ping_encrypted, tr_enc) -> (
-      (* If encryption succeeds, we get a new trace `tr_enc`.
-         With the lemma `pke_enc_for_invariant` in `DY.Simplified`,
-         we have that trace_invariant holds for tr_enc.
-
-         Observe, that this lemma can be shown automatically.
-         Hence, we don't even have to call it here.
-      *)
-      assert(trace_invariant tr_enc);
-
-      (* The next traceful action is sending the encrypted message.
-
-         Again, we have to pass the current trace `tr_enc` as last argument.
-      *)
-      let (msg_ts, tr_msg) = send_msg ping_encrypted tr_enc in
-      (* To show trace_invariant after sending the message (for `tr_msg`),
-         we look at the lemma `send_msg_invariant` in `DY.Core.Trace.Manipulation`
-         which looks very promising.
-         However, that lemma has an additional pre-condition requiring that
-         the message needs to be publishable.
-         (That corresponds to the intuition that everything on the trace 
-         is readable by the attacker.)
-
-         So to call this lemma, we have to show `is_publishable tr_enc ping_encrypted`.
-         Looking at `DY.Simplified`, we find the lemma `pke_enc_for_is_publishable`,
-         which gives a bunch of pre-conditions for the plaintext (serialized `ping`) 
-         under which the ciphertext `ping_encrypted` is publishable.
-         We show each of those pre-conditions.
-      *)
-          (* The first is `has_pki_invariant`.
-
-             It is a technical requirement on the protocol invariants 
-             which we are not explaining here.
-
-             In `DY.OnlineS.Invariants` we have the lemma `protocol_invariants_p_has_pki_invariant`
-             showing this requirement.
-          *)
-          assert(has_pki_invariant);
-
-          (* The next requirement for `pke_enc_for_is_publishable` is `bytes_invariant tr_enc (serialize ping)`.
-
-             TODO              
-          *)
-          serialize_wf_lemma message_t (is_knowable_by (nonce_label alice bob) tr_sess) ping;
-
-          (* The next two pre-conditions say
-             that the serialized ping should be readable by Alice and Bob.
-             (Ignore the `long_term_key_label` for now.)
-
-             TODO: they are resolved with the same serialize_wf_lemma
-          *)
-
-          (* Finally, we need to show the disjunction of
-             * the pke_pred holds for the serialized ping or
-             * the serialized ping is publishable
-
-             In our case, the first is true, i.e., the encryption prediate is satisfied.
-             The predicate requires that the nonce contained in the ping
-             has the label `nonce_label alice' bob'`, where
-             * alice' is the name in the first component of the ping and
-             * bob' is the participant whos key is used for encryption.
-
-             Since we generate the nonce n_a in the beginning of this step
-             with the label `nonce_label alice bob`,
-             put the same alice in the first component of the ping
-             and use the key of bob for encryption (in pke_enc_for),
-             we satisfy the predicate.
-          *)
-          assert(pke_pred.pred tr_sess (long_term_key_type_to_usage (LongTermPkeKey key_tag) bob) (serialize message_t ping));
-      (* Now we showed all pre-conditions of `pke_enc_for_is_publishable`
-         and can call this lemma to show that ping_encrypted is publishable.
-
-         Together with the `send_msg_invariant` lemma, 
-         we then obtain that `tr_msg` satisfies the trace invariant.
-      *)
-      pke_enc_for_is_publishable tr_sess alice bob keys_sid key_tag ping;
-      assert(trace_invariant tr_msg);
-
-   ()  
-  )
-
-(* The above proof was very detailed.
-   In fact, most of the proof is done automatically by F*
-   and we can remove all of the asserts.
-
-   If we just keep the necessary calls to lemmas,
-   we end up with the following very short proof.
-*)
 val send_ping_invariant_short_version:
   alice:principal -> bob:principal -> keys_sid:state_id ->
   tr:trace ->
@@ -222,6 +36,10 @@ val send_ping_invariant_short_version:
   ))
 let send_ping_invariant_short_version alice bob keys_sid  tr =
   let (n_a, tr_rand) = gen_rand_labeled (nonce_label alice bob) tr in
+  (* We have to adapt the proof to the new send_ping function,
+     i.e., we triggered an event and
+     swapped the order of storing the state and sending the message
+  *)
   let (_, tr_ev) = trigger_event alice (Initiating {alice; bob; n_a}) tr_rand in
   let (_, tr_sess) = start_new_session alice (SendingPing {bob; n_a}) tr_ev in  
   let ping = Ping {alice; n_a} in 
@@ -230,14 +48,6 @@ let send_ping_invariant_short_version alice bob keys_sid  tr =
 
 
 (*** Replying to a Ping maintains the invariants ***)
-
-
-(* For the second protocol step (`receive_ping_and_send_ack`),
-   we need a helper lemma: `decode_ping_proof`.
-
-   Ignore this for now, and jump to the next lemma 
-   `receive_ping_and_send_ack_invariant`
-*)
 
 val decode_ping_proof:
   tr:trace ->
@@ -285,104 +95,60 @@ val receive_ping_and_send_ack_invariant:
     trace_invariant tr_out
   ))
 let receive_ping_and_send_ack_invariant bob bob_keys_sid msg_ts tr =
-  (* As for the first protocol step,
-     we need to show that every traceful action 
-     maintains the trace invariant.
-  *)
-  match recv_msg msg_ts tr with // unfold the traceful + option let
-  | (None, _ ) -> () // in this case the trace is not changed and hence the trace invariant is trivially satisfied
+  match recv_msg msg_ts tr with
+  | (None, _ ) -> ()
   | (Some msg, _) -> (
-      (* From the lemma `recv_msg_same_trace` in `DY.Core.Trace.Manipulation` 
-         we have that the receive function does not change the trace
-         and hence the trace invariant is still satisfied. *)
-      match decode_ping bob bob_keys_sid.private_keys msg tr with // unfold the next monadic let
-      | (None, _) -> () // Again, if decoding fails, the trace is not changed and hence nothing left to show
+      match decode_ping bob bob_keys_sid.private_keys msg tr with
+      | (None, _) -> ()
       | (Some png, _) -> (
-          (* Decoding the ping message does not change the trace.
-             So we are still working on the input trace tr,
-             for which we know the trace invariant.
-
-             That decoding doesn't change the trace,
-             is shown automatically 
-             with corresponding SMT patterns for the individual steps of the function.
-             I.e., try uncommenting the following lemma:
-           *) 
-             // let decode_ping_same_trace
-             //    (p:principal) (keys_sid:state_id) (msg:bytes) (tr:trace) :
-             //    Lemma (
-             //       let (_, tr_out) = decode_ping p keys_sid msg tr in
-             //       tr_out == tr )
-             //    = () in
-          
           let n_a = png.n_a in
           let alice = png.alice in
           
           let ack = Ack {n_a} in
 
- (* As in the first protocol step,
-                   starting a new session maintains the trace invariant,
-                   if the new state satisfies the state predicate.
+          (* Again, we have to adapt the proof to the new order of
+             first storing the state and then sending the message.
 
-                   For the new SendingAck state, this means that
-                   the stored nonce
-                   must be readble by
-                   the storing principal (here bob).
+             The proof that this step maintains the invariant,
+             is the same as before:
+             
+             starting a new session maintains the trace invariant,
+             if the new state satisfies the state predicate.
 
-                   We get this property from our helper lemma `decode_ping_proof`.
-                *)
-                let st = (SendingAck {alice = png.alice; n_a = png.n_a}) in
-                let (sess_id, tr_sess) = start_new_session bob st tr in
-                                  decode_ping_proof tr bob bob_keys_sid.private_keys msg;
+             For the new SendingAck state, this means that
+             the stored nonce
+             must be readble by
+             the storing principal (here bob).
 
-                assert(trace_invariant tr_sess);
+             And that there is some alice, that
+             stored a SendinPing state,
+             unless the nonce n_a is publishable.
 
+             We get this property from our helper lemma `decode_ping_proof`:
+             which says:
+             the nonce n_a is publishable,
+             or we get the guarantees from the pke_pred for the decoded Ping.
+             From the pke_pred, we get that 
+             alice contained in the Ping stored a SendingPing state.
+          *)
+          let st = (SendingAck {alice = png.alice; n_a = png.n_a}) in
+          let (sess_id, tr_sess) = start_new_session bob st tr in
+          decode_ping_proof tr bob bob_keys_sid.private_keys msg;
+          assert(trace_invariant tr_sess);
+
+          (* The rest of the proof is the same as before. *)
           match pke_enc_for bob alice bob_keys_sid.pki key_tag ack tr_sess with
           | (None, _) -> ()
           | (Some ack_encrypted, tr_ack) ->(
-                (* As before, encryption maintains the trace invariant 
-                   (see `pke_enc_for_invariant` in `DY.simplified`) *)
                 assert(trace_invariant tr_ack);
 
                 let (ack_ts, tr_msg) = send_msg ack_encrypted tr_ack in
-                (* The same as in the first protocol step:
-                   we want to use the lemma `send_msg_invariant` from `DY.Core.Trace.Manipulation`
-                   to show that sending the encrypted ack maintains the invariant.
-
-                   For this, we need to show that the encrypted ack is publishable.
-                   Again, we want to apply the lemma `pke_enc_for_is_publishable` from `DY.Simplified`.
-                   So we have to show all of the pre-conditions of this lemma.
-                *)
-                  (* `trace_invariant tr` and `has_pki_invariant` are satisfied *)
-                  (* For `bytes_invariant` of the serialized ack,
-                     we need a helper lemma.
-
-                     TODO ....
-                  *)
-                  decode_ping_proof tr bob bob_keys_sid.private_keys msg;
                   serialize_wf_lemma message_t (bytes_invariant tr) (ack);
-                  assert(bytes_invariant tr (serialize message_t ack));
-                  
-                  (* From this helper lemma, we also get
-                     that the nonce is readable by alice and bob.
-
-                     We use this fact together with a comparse lemma,
-                     to show the next two requirements:
-                     the serialized ack is readable by alice and bob 
-                     (again ignoring the `long_term_key_label`) *)
+                  assert(bytes_invariant tr (serialize message_t ack));                  
                   assert(is_knowable_by (nonce_label alice bob) tr n_a);
                   serialize_wf_lemma message_t (is_knowable_by (nonce_label alice bob) tr) ack;
-
-                  (* The final requirement is trivially satisfied, 
-                     since the pke_pred for an Ack is just True
-
-                     You can check:
-                     assert(pke_pred.pred tr (long_term_key_type_to_usage (LongTermPkeKey key_tag) alice) (serialize message_t ack));
-                  *)
-                (* Thus, we can call `pke_enc_for_is_publishable`
-                   to get the missing pre-condition for `send_msg_invariant`.*)
                 pke_enc_for_is_publishable tr_sess bob alice bob_keys_sid.pki key_tag ack;
                 assert(trace_invariant tr_msg);
-
                ()
            )
       )
@@ -391,6 +157,13 @@ let receive_ping_and_send_ack_invariant bob bob_keys_sid msg_ts tr =
 
 
 (*** Receiving an Ack maintains the invariants ***)
+
+
+/// Since we now have a non-trivial property for the ReceivedAck state,
+/// the proof does not work automatically anymore (as it did for the secrecy model).
+///
+/// In the same manner as for the other functions,
+/// we need a helper lemma for decoding an ack.
 
 val decode_ack_proof:
   tr:trace ->
@@ -407,7 +180,6 @@ val decode_ack_proof:
     | (Some ack, _) -> (
         let n_a = ack.n_a in
         bytes_invariant tr n_a /\
-        //is_knowable_by (principal_label alice) tr n_a /\
         ( is_publishable tr n_a
         \/ (pke_pred.pred tr (long_term_key_type_to_usage (LongTermPkeKey key_tag) alice) (serialize message_t (Ack ack)))
         )
@@ -425,11 +197,25 @@ let decode_ack_proof tr alice keys_sid msg =
     )
   
 
+/// Additionally,
+/// we need an injectivity lemma.
+/// The goal is to show that Alice uses the nonces n_a
+/// only once, i.e., the nonce n_a are unique for every run.
+///
+/// We show this with the help of the Initiating event:
+/// If there are two events triggered by the same Alice
+/// using the same nonce n_a,
+/// then the contained other participants (Bob) must also be the same.
+///
+/// The proof is automatic from the event prediate,
+/// which says that the contained nonce n_a
+/// was generated right before the event.
+/// Since nonces are uniquely identified by their time of creation,
+/// this immediately shows that
+/// two events referring to the same nonce,
+/// must be the same event.
 
-/// The invariant lemma for the final protocol step `receive_ack_invariant`
-
-
-val event_respond1_injective:
+val event_initiating_injective:
   tr:trace ->
   alice:principal -> bob:principal -> bob':principal ->
   n_a:bytes ->
@@ -442,8 +228,26 @@ val event_respond1_injective:
   (ensures
     bob == bob'
   )
-let event_respond1_injective tr alice bob bob' n_a = ()
+let event_initiating_injective tr alice bob bob' n_a = ()
 
+val event_initiating_injective_:
+  tr:trace ->
+  alice:principal -> alice':principal -> bob:principal -> bob':principal ->
+  n_a:bytes ->
+  Lemma
+  (requires
+    trace_invariant tr /\
+    event_triggered tr alice (Initiating {alice; bob; n_a} ) /\
+    event_triggered tr alice' (Initiating {alice =alice'; bob =bob'; n_a} )
+  )
+  (ensures
+    alice == alice' /\
+    bob == bob'
+  )
+let event_initiating_injective_ tr alice alice' bob bob' n_a = ()
+
+
+/// The invariant lemma for the final protocol step `receive_ack_invariant`
 
 #push-options "--ifuel 2"
 val receive_ack_invariant:
@@ -457,7 +261,6 @@ val receive_ack_invariant:
     let (_, tr_out) = receive_ack alice keys_sid msg_ts tr in
     trace_invariant tr_out
   ))
-(* The proof for this last step is automatic. *)
 let receive_ack_invariant alice keys_sid msg_ts tr =
   match recv_msg msg_ts tr with
   | (None, _) -> ()
@@ -474,25 +277,40 @@ let receive_ack_invariant alice keys_sid msg_ts tr =
               let newst = ReceivedAck {bob; n_a} in
 
               let ((), tr_st) = set_state alice sid newst tr in
+              // We show the state predicate for the new ReceivedAck state in the following
 
-              assert(event_triggered tr alice (Initiating {alice; bob;n_a}));
+              // from the SendPing state predicate
               assert(is_secret (nonce_label alice bob) tr n_a);
+              // immediate consequence of the exact label of n_a
               assert(is_publishable tr n_a ==> is_corrupt tr (principal_label alice) \/ is_corrupt tr (principal_label bob));
-              introduce ~(is_publishable tr n_a) ==> 
-            state_was_set_some_id tr bob (SendingAck {alice; n_a} )
-            with _. (
-              decode_ack_proof tr alice keys_sid msg;
-              assert(pke_pred.pred tr (long_term_key_type_to_usage (LongTermPkeKey key_tag) alice) (serialize message_t (Ack ack)));
-              eliminate exists bob'. get_label tr n_a `can_flow tr` (principal_label bob') /\ 
-              state_was_set_some_id tr bob' (SendingAck {alice; n_a} )
-              returns _
-              with _. (
-                assert(event_triggered tr alice (Initiating {alice; bob = bob'; n_a} ));
-                event_respond1_injective tr alice bob bob' n_a
-              
-              )
 
-            );
+              (* the more difficult case is the honest case,
+                 when the nonce is not publishable
+              *)
+              introduce ~(is_publishable tr n_a) ==> state_was_set_some_id tr bob (SendingAck {alice; n_a} )
+              with _. (
+                decode_ack_proof tr alice keys_sid msg;
+                (* From the pke_pred for the decoded Ack,
+                   we get that there is some bob' that set a SendingAck state.
+                   So, we need to show, that this bob' is 
+                   the same as the bob stored in Alice's SendPing state.
+
+                   We get this from the nonce injectivity from above.
+                *)
+                assert(pke_pred.pred tr (long_term_key_type_to_usage (LongTermPkeKey key_tag) alice) (serialize message_t (Ack ack)));
+                eliminate exists bob'. state_was_set_some_id tr bob' (SendingAck {alice; n_a})
+                returns _
+                with _. (
+                  // from the state predicate of the looked up SendingPing state of Alice:
+                  assert(event_triggered tr alice (Initiating {alice; bob;n_a}));
+
+                  // from the state predicate of the SendingAck state of bob':
+                  assert(event_triggered tr alice (Initiating {alice; bob = bob'; n_a} ));
+
+                  // the injectivity lemma from above, yields bob' = bob
+                  event_initiating_injective tr alice bob bob' n_a
+                )
+              );
               assert(trace_invariant tr_st)
           )
       )
