examples/Online_with_authn/DY.OnlineA.Invariants.fst
@@ -24,68 +24,57 @@ open DY.OnlineA.Protocol
 /// With this, we then know that
 /// the protocol model satisfies the secrecy property.
 
+/// We highlight only the differences to
+/// the invariants for the nonce secrecy proof (Online_with_secrecy/DY.OnlineS.Invariants.fst)
+/// 
 
 (*** Crypto Invariants ***)
 
 
-(** TODO **)
-// needed for `crypto_prediates.pke_pred.pred_later`
 %splice [ps_ping_t_is_well_formed] (gen_is_well_formed_lemma (`ping_t))
 %splice [ps_ack_t_is_well_formed] (gen_is_well_formed_lemma (`ack_t))
 %splice [ps_message_t_is_well_formed] (gen_is_well_formed_lemma (`message_t))
 
-
-
-// ignore this for now
 instance crypto_usages_p : crypto_usages = default_crypto_usages
 
 #push-options "--ifuel 2"
 let crypto_p : crypto_predicates = { 
   default_crypto_predicates with 
-  (* we restrict when a message is allowed to be encrypted 
-     with some secret key
-
-     Or put differently:
-     What are the guarantees that an honest sender can provide
-     that are available at the receiver after decryption?
-  *)
   pke_pred = { 
     pred = (fun tr sk_usage msg ->
-    exists prin. // the intended receiver of the message
+    exists prin.
     (
-      // needed for `decode_ping_proof` [Why?]
-      (* the key used for the encryption is
-         a protocol-level public key for the intended receiver (prin) 
-      *)
       sk_usage == long_term_key_type_to_usage (LongTermPkeKey key_tag) prin /\
       (match parse message_t msg with
       | Some (Ping ping) ->
-          (* a Ping message can only be encrypted if
-             (Or: if you decrypt a Ping from an honest party 
-             you get the guarantees that:)
-             the contained nonce n_a
-             is labeled for 
-             * the name provided in the message (alice)
-             * and the intended receiver of the message (bob)
-          *)
           let bob = prin in
           let alice = ping.alice in
           let n_a = ping.n_a in
           get_label tr n_a == nonce_label alice bob
+          (* additionally, we here also require/guarantee
+             that the principal in the message (alice)
+             stored a SendingPing state before sendind the message,
+             containing:
+             * the intended receiver (bob) and
+             * the nonce in the message (n_a)
+          *)
           /\ state_was_set_some_id tr alice (SendingPing {bob; n_a})
       | Some (Ack ack) ->
           let alice = prin in
           let n_a = ack.n_a in
+          (* In contrast to the secrecy proof,
+             where we didn't need any guarantees for an Ack message,
+             we here have the property that
+             there is some principal bob that 
+             stored a SendingAck state with 
+             * the intended receiver of the Ack (alice) and
+             * the nonce in the Ack (n_a)
+          *)
           exists bob.
-          state_was_set_some_id tr bob (SendingAck {alice = prin; n_a = ack.n_a})
-          /\ get_label tr n_a `can_flow tr` principal_label bob
-      | _ -> False // other messages can not be encrypted
+            state_was_set_some_id tr bob (SendingAck {alice = prin; n_a = ack.n_a})
+      | _ -> False
       ))
       ); 
-    (* a lemma guaranteeing:
-       if the predicate specified above holds for some trace tr1
-       it also holds for any extension tr2 of tr1
-    *)
     pred_later = (fun tr1 tr2 pk msg -> 
       parse_wf_lemma message_t (bytes_well_formed tr1) msg
     ) 
@@ -103,46 +92,45 @@ instance crypto_invariants_p: crypto_invariants = {
 
 (*** State Invariant ***)
 
-// TODO
-// Needed for `state_predicate.pred_knowable`
 %splice [ps_sent_ping_t_is_well_formed] (gen_is_well_formed_lemma (`sent_ping_t))
 %splice [ps_sent_ack_t_is_well_formed] (gen_is_well_formed_lemma (`sent_ack_t))
 %splice [ps_received_ack_t_is_well_formed] (gen_is_well_formed_lemma (`received_ack_t))
 %splice [ps_state_t_is_well_formed] (gen_is_well_formed_lemma (`state_t))
 
-#push-options "--z3cliopt 'smt.qi.eager_threshold=50'"
-(* We restrict what states are allowed to be stored by principals *)
+#push-options "--ifuel 2 --z3cliopt 'smt.qi.eager_threshold=50'"
 let state_predicate_p: local_state_predicate state_t = {
   pred = (fun tr prin sess_id st ->
     match st with
     | SendingPing ping -> (
-        (* a SendingPing state may only be stored if
-           the stored nonce is labeled for
-           * the storing principal (alice)
-           * the principal stored in the state 
-             (the intended receiver of the Ping: bob)
-        *) 
         let alice = prin in
         let bob = ping.bob in
         let n_a = ping.n_a in
         is_secret (nonce_label alice bob) tr n_a
+        (* additionally to the secrecy proof,
+           we add the property that 
+           the storing principal (alice)
+           triggered in Initiating event containing:
+           * her own name
+           * the principal stored in the state (bob) and
+           * the nonce stored in the state (n_a)
+        *) 
         /\ event_triggered tr alice (Initiating {alice = alice; bob = bob; n_a = n_a})
     )
     | SendingAck ack -> (
-        (* a SendingAck state may only be stored if
-           the stored nonce is readable by
-           the storing principal (bob)
-
-           -- this is a condition that must always hold,
-           and is enforced by the `pred_knowable` Lemma.
-        *)
         let bob = prin in
         let n_a = ack.n_a in
         is_knowable_by (principal_label bob) tr n_a
-        /\ (exists alice.
-          //is_corrupt tr (principal_label alice) \/
+        (* here we add,
+           that the stored other principal (alice)
+           stored a SendingPing state containing
+           * the current storing principal (bob) and
+           * the nonce stored in the state (n_a)
+           except, if we are in the case that 
+           the stored nonce (n_a) has leaked to the attacker.
+        *)
+        /\ (
           is_publishable tr n_a \/
-          event_triggered tr alice (Initiating {alice; bob; n_a})
+          state_was_set_some_id tr ack.alice (SendingPing {bob; n_a})
         )
     )
     | ReceivedAck rack  -> (
@@ -155,38 +143,49 @@ let state_predicate_p: local_state_predicate state_t = {
         let alice = prin in
         let bob = rack.bob in
         let n_a = rack.n_a in
-        is_knowable_by (principal_label alice) tr n_a /\
+        is_secret (nonce_label alice bob) tr n_a /\
 
+        (* this is already the authentication property we want to show:
+           alice stores a ReceivedAck state only, if
+           the stored principal (bob) stored a SendingAck state containing:
+           * alice and
+           * the nonce n_a
+           unless,
+           one of alice or bob are corrupt
+        *)
         (state_was_set_some_id tr bob (SendingAck {alice; n_a})
         \/ (is_corrupt tr (principal_label alice) \/ is_corrupt tr (principal_label bob)))
     )
   );
-  (* as for encryption we have a lemma guaranteeing:
-     if the state predicate holds on some trace tr1
-     it also holds for any extension tr2 of tr2
-  *)
   pred_later = (fun tr1 tr2 prin sess_id st -> () );
-  (* a lemma guaranteeing that
-     the content of the state to be stored
-     is readable by the storing principal
-  *)
-  pred_knowable = (fun tr prin sess_id st -> 
-    match st with
-    | SendingAck ack -> ()
-    | _ -> ()
-  );
+  pred_knowable = (fun tr prin sess_id st -> () );
 }
 #pop-options
 
 (*** Event Pred ***)
 
+/// As for messages and states,
+/// we also have prediates on events.
+/// The intuition is similar:
+/// They say when an event is allowed to be triggered, or
+/// what guarantees we obtain, if we observe an event on the trace.
+
 let event_predicate_event_t: event_predicate event_t =
   fun tr prin e ->
+  // prin is the principal triggering the event
     match e with    
     | Initiating init -> (
         let alice = init.alice in
         let bob = init.bob in
         let n_a = init.n_a in
+        (* We may trigger the Initiating event only if,
+           * the triggering principal is the first principal stored in the event (alice)
+           * the nonce (n_a) in the event is labelled for 
+             the two principals stored in the event (alice and bob)
+           * the stored nonce (n_a) was generated right before the event is triggered
+             (this is crucial and will be used to show an injectivity property,
+             that there will be only one such event for a fixed nonce n_a)
+        *)
         prin == alice /\
         is_secret (nonce_label alice bob) tr n_a /\
         0 < DY.Core.Trace.Base.length tr /\
@@ -195,15 +194,13 @@ let event_predicate_event_t: event_predicate event_t =
 
 (*** Trace invariants ***)
 
-// TODO: can this (all_sessions and all_events) be hidden somehow?
 let all_sessions = [
   pki_tag_and_invariant;
   private_keys_tag_and_invariant;
   (|local_state_state.tag, local_state_predicate_to_local_bytes_state_predicate state_predicate_p|);
 ]
 
-/// We have no events here,
-/// but we need to specify that for the trace invariants
+/// Now we have an event type
 let all_events = [(event_event_t.tag, compile_event_pred event_predicate_event_t)]
 
 
@@ -231,9 +228,7 @@ instance protocol_invariants_p: protocol_invariants = {
 }
 
 
-(*** Helper Lemmas for the Secrecy Proof ***)
-
-// TODO: Can all of this be hidden somehow?
+(*** Helper Lemmas ***)
 
 val all_sessions_has_all_sessions: unit -> Lemma (norm [delta_only [`%all_sessions; `%for_allP]; iota; zeta] (for_allP (has_local_bytes_state_predicate) all_sessions))
 let all_sessions_has_all_sessions () =
@@ -250,6 +245,8 @@ let protocol_invariants_p_has_pki_invariant = all_sessions_has_all_sessions ()
 val protocol_invariants_p_has_private_keys_invariant: squash (has_private_keys_invariant #protocol_invariants_p)
 let protocol_invariants_p_has_private_keys_invariant = all_sessions_has_all_sessions ()
 
+/// We need similar lemmas for our event type
+
 val all_events_has_all_events: unit -> Lemma (norm [delta_only [`%all_events; `%for_allP]; iota; zeta] (for_allP (has_compiled_event_pred #protocol_invariants_p) all_events))
 let all_events_has_all_events () =
   assert_norm(List.Tot.no_repeats_p (List.Tot.map fst (all_events)));
@@ -258,6 +255,5 @@ let all_events_has_all_events () =
   let dumb_lemma (x:prop) (y:prop): Lemma (requires x /\ x == y) (ensures y) = () in
   dumb_lemma (for_allP (has_compiled_event_pred #protocol_invariants_p) all_events) (norm [delta_only [`%all_events; `%for_allP]; iota; zeta] (for_allP (has_compiled_event_pred #protocol_invariants_p) all_events))
 
-// As an example, below `#protocol_invariants_nsl` is omitted and instantiated using F*'s typeclass resolution algorithm
-val protocol_invariants_nsl_has_nsl_event_invariant: squash (has_event_pred event_predicate_event_t)
-let protocol_invariants_nsl_has_nsl_event_invariant = all_events_has_all_events ()
+val protocol_invariants_p_has_event_t_invariant: squash (has_event_pred event_predicate_event_t)
+let protocol_invariants_p_has_event_t_invariant = all_events_has_all_events ()
